test_databases/compressed_phase/evil_duplicate_save.mm
@@ -1,0 +1,8 @@
+$c |- p $.
+ax $a |- p $.
+${
+  left $e |- p $.
+  right $e |- p $.
+  merge $a |- p $.
+$}
+evilClone $p |- p $= ( ax merge ) AZZDB $.
