test_databases/compressed_phase/evil_mandatory_header_hyp.mm
@@ -1,0 +1,5 @@
+$c wff |- $.
+$v x $.
+wx $f wff x $.
+ax $a |- x $.
+evil $p |- x $= ( wx ax ) BC $.
