test_databases/compressed_phase/evil_unknown_interrupt.mm
@@ -1,0 +1,3 @@
+$c |- p $.
+ax $a |- p $.
+evilUnknown $p |- p $= ( ax ) AU? $.
