test_databases/compressed_phase/positive_nonmandatory_header_hyp.mm
@@ -1,0 +1,6 @@
+$c wff |- $.
+$v x y $.
+wx $f wff x $.
+wy $f wff y $.
+ax $a |- x $.
+good $p |- x $= ( wy ax ) AC $.
