test_databases/compressed_phase/positive_single_save.mm
@@ -1,0 +1,8 @@
+$c |- p $.
+ax $a |- p $.
+${
+  left $e |- p $.
+  right $e |- p $.
+  merge $a |- p $.
+$}
+positive $p |- p $= ( ax merge ) AZCB $.
